---
layout: page
title: "Function extensionality"
category: lemmas functions homotopy
toc: true
agda: true
gallery: true
latex: true
references: true
linkify: true
showcitation: true
home: true
---

<div class="hide" >
<pre class="Agda">
<a id="233" class="Symbol">{-#</a> <a id="237" class="Keyword">OPTIONS</a> <a id="245" class="Pragma">--without-K</a> <a id="257" class="Symbol">#-}</a>
<a id="261" class="Keyword">open</a> <a id="266" class="Keyword">import</a> <a id="273" href="Transport.html" class="Module">Transport</a>
<a id="283" class="Keyword">open</a> <a id="288" class="Keyword">import</a> <a id="295" href="EquivalenceType.html" class="Module">EquivalenceType</a>
<a id="311" class="Keyword">open</a> <a id="316" class="Keyword">import</a> <a id="323" href="HomotopyType.html" class="Module">HomotopyType</a>
</pre>
</div>

## Function extensionality

<pre class="Agda">

<a id="397" class="Keyword">module</a> <a id="404" href="FunExtAxiom.html" class="Module">FunExtAxiom</a> <a id="416" class="Symbol">{</a><a id="417" href="FunExtAxiom.html#417" class="Bound">ℓᵢ</a> <a id="420" href="FunExtAxiom.html#420" class="Bound">ℓⱼ</a><a id="422" class="Symbol">}</a> <a id="424" class="Symbol">{</a><a id="425" href="FunExtAxiom.html#425" class="Bound">A</a> <a id="427" class="Symbol">:</a> <a id="429" href="Intro.html#1442" class="Function">Type</a> <a id="434" href="FunExtAxiom.html#417" class="Bound">ℓᵢ</a><a id="436" class="Symbol">}</a>
  <a id="440" class="Symbol">{</a><a id="441" href="FunExtAxiom.html#441" class="Bound">B</a> <a id="443" class="Symbol">:</a> <a id="445" href="FunExtAxiom.html#425" class="Bound">A</a> <a id="447" class="Symbol">→</a> <a id="449" href="Intro.html#1442" class="Function">Type</a> <a id="454" href="FunExtAxiom.html#420" class="Bound">ℓⱼ</a><a id="456" class="Symbol">}</a> <a id="458" class="Symbol">{</a><a id="459" href="FunExtAxiom.html#459" class="Bound">f</a> <a id="461" href="FunExtAxiom.html#461" class="Bound">g</a> <a id="463" class="Symbol">:</a> <a id="465" class="Symbol">(</a><a id="466" href="FunExtAxiom.html#466" class="Bound">a</a> <a id="468" class="Symbol">:</a> <a id="470" href="FunExtAxiom.html#425" class="Bound">A</a><a id="471" class="Symbol">)</a> <a id="473" class="Symbol">→</a> <a id="475" href="FunExtAxiom.html#441" class="Bound">B</a> <a id="477" href="FunExtAxiom.html#466" class="Bound">a</a><a id="478" class="Symbol">}</a> <a id="480" class="Keyword">where</a>
</pre>

<pre class="Agda">
  <a id="513" class="Comment">-- Application of an homotopy</a>
  <a id="happly"></a><a id="545" href="FunExtAxiom.html#545" class="Function">happly</a>
    <a id="556" class="Symbol">:</a> <a id="558" href="FunExtAxiom.html#459" class="Bound">f</a> <a id="560" href="EqualityType.html#931" class="Datatype Operator">==</a> <a id="563" href="FunExtAxiom.html#461" class="Bound">g</a>
    <a id="569" class="Comment">------------------------</a>
    <a id="598" class="Symbol">→</a> <a id="600" class="Symbol">((</a><a id="602" href="FunExtAxiom.html#602" class="Bound">x</a> <a id="604" class="Symbol">:</a> <a id="606" href="FunExtAxiom.html#425" class="Bound">A</a><a id="607" class="Symbol">)</a> <a id="609" class="Symbol">→</a> <a id="611" href="FunExtAxiom.html#459" class="Bound">f</a> <a id="613" href="FunExtAxiom.html#602" class="Bound">x</a> <a id="615" href="EqualityType.html#931" class="Datatype Operator">==</a> <a id="618" href="FunExtAxiom.html#461" class="Bound">g</a> <a id="620" href="FunExtAxiom.html#602" class="Bound">x</a><a id="621" class="Symbol">)</a>

  <a id="626" href="FunExtAxiom.html#545" class="Function">happly</a> <a id="633" href="EqualityType.html#985" class="InductiveConstructor">idp</a> <a id="637" href="FunExtAxiom.html#637" class="Bound">x</a> <a id="639" class="Symbol">=</a> <a id="641" href="EqualityType.html#1111" class="Function">refl</a> <a id="646" class="Symbol">(</a><a id="647" href="FunExtAxiom.html#459" class="Bound">f</a> <a id="649" href="FunExtAxiom.html#637" class="Bound">x</a><a id="650" class="Symbol">)</a>
</pre>

<pre class="Agda">
  <a id="679" class="Keyword">postulate</a>
    <a id="axiomFunExt"></a><a id="693" href="FunExtAxiom.html#693" class="Postulate">axiomFunExt</a> <a id="705" class="Symbol">:</a> <a id="707" href="EquivalenceType.html#622" class="Function">isEquiv</a> <a id="715" href="FunExtAxiom.html#545" class="Function">happly</a>
</pre>

<pre class="Agda">
  <a id="eqFunExt"></a><a id="749" href="FunExtAxiom.html#749" class="Function">eqFunExt</a>
    <a id="762" class="Symbol">:</a> <a id="764" class="Symbol">(</a><a id="765" href="FunExtAxiom.html#459" class="Bound">f</a> <a id="767" href="EqualityType.html#931" class="Datatype Operator">==</a> <a id="770" href="FunExtAxiom.html#461" class="Bound">g</a><a id="771" class="Symbol">)</a> <a id="773" href="EquivalenceType.html#778" class="Function Operator">≃</a> <a id="775" class="Symbol">((</a><a id="777" href="FunExtAxiom.html#777" class="Bound">x</a> <a id="779" class="Symbol">:</a> <a id="781" href="FunExtAxiom.html#425" class="Bound">A</a><a id="782" class="Symbol">)</a> <a id="784" class="Symbol">→</a> <a id="786" href="FunExtAxiom.html#459" class="Bound">f</a> <a id="788" href="FunExtAxiom.html#777" class="Bound">x</a> <a id="790" href="EqualityType.html#931" class="Datatype Operator">==</a> <a id="793" href="FunExtAxiom.html#461" class="Bound">g</a> <a id="795" href="FunExtAxiom.html#777" class="Bound">x</a><a id="796" class="Symbol">)</a>

  <a id="801" href="FunExtAxiom.html#749" class="Function">eqFunExt</a> <a id="810" class="Symbol">=</a> <a id="812" href="FunExtAxiom.html#545" class="Function">happly</a> <a id="819" href="BasicTypes.html#1479" class="InductiveConstructor Operator">,</a> <a id="821" href="FunExtAxiom.html#693" class="Postulate">axiomFunExt</a>
</pre>

<pre class="Agda">
  <a id="860" class="Comment">-- From this, the usual notion of function extensionality follows.</a>
  <a id="funext"></a><a id="929" href="FunExtAxiom.html#929" class="Function">funext</a>
    <a id="940" class="Symbol">:</a> <a id="942" class="Symbol">((</a><a id="944" href="FunExtAxiom.html#944" class="Bound">x</a> <a id="946" class="Symbol">:</a> <a id="948" href="FunExtAxiom.html#425" class="Bound">A</a><a id="949" class="Symbol">)</a> <a id="951" class="Symbol">→</a> <a id="953" href="FunExtAxiom.html#459" class="Bound">f</a> <a id="955" href="FunExtAxiom.html#944" class="Bound">x</a> <a id="957" href="EqualityType.html#931" class="Datatype Operator">==</a> <a id="960" href="FunExtAxiom.html#461" class="Bound">g</a> <a id="962" href="FunExtAxiom.html#944" class="Bound">x</a><a id="963" class="Symbol">)</a>
    <a id="969" class="Comment">------------------------</a>
    <a id="998" class="Symbol">→</a> <a id="1000" href="FunExtAxiom.html#459" class="Bound">f</a> <a id="1002" href="EqualityType.html#931" class="Datatype Operator">==</a> <a id="1005" href="FunExtAxiom.html#461" class="Bound">g</a>

  <a id="1010" href="FunExtAxiom.html#929" class="Function">funext</a> <a id="1017" class="Symbol">=</a> <a id="1019" href="EquivalenceType.html#1147" class="Function">remap</a> <a id="1025" href="FunExtAxiom.html#749" class="Function">eqFunExt</a>
</pre>

<pre class="Agda">
  <a id="1061" class="Comment">-- Beta and eta rules for function extensionality</a>
  <a id="funext-β"></a><a id="1113" href="FunExtAxiom.html#1113" class="Function">funext-β</a>
    <a id="1126" class="Symbol">:</a> <a id="1128" class="Symbol">(</a><a id="1129" href="FunExtAxiom.html#1129" class="Bound">h</a> <a id="1131" class="Symbol">:</a> <a id="1133" class="Symbol">((</a><a id="1135" href="FunExtAxiom.html#1135" class="Bound">x</a> <a id="1137" class="Symbol">:</a> <a id="1139" href="FunExtAxiom.html#425" class="Bound">A</a><a id="1140" class="Symbol">)</a> <a id="1142" class="Symbol">→</a> <a id="1144" href="FunExtAxiom.html#459" class="Bound">f</a> <a id="1146" href="FunExtAxiom.html#1135" class="Bound">x</a> <a id="1148" href="EqualityType.html#931" class="Datatype Operator">==</a> <a id="1151" href="FunExtAxiom.html#461" class="Bound">g</a> <a id="1153" href="FunExtAxiom.html#1135" class="Bound">x</a><a id="1154" class="Symbol">))</a>
    <a id="1161" class="Comment">------------------------------</a>
    <a id="1196" class="Symbol">→</a> <a id="1198" href="FunExtAxiom.html#545" class="Function">happly</a> <a id="1205" class="Symbol">(</a><a id="1206" href="FunExtAxiom.html#929" class="Function">funext</a> <a id="1213" href="FunExtAxiom.html#1129" class="Bound">h</a><a id="1214" class="Symbol">)</a> <a id="1216" href="EqualityType.html#931" class="Datatype Operator">==</a> <a id="1219" href="FunExtAxiom.html#1129" class="Bound">h</a>

  <a id="1224" href="FunExtAxiom.html#1113" class="Function">funext-β</a> <a id="1233" href="FunExtAxiom.html#1233" class="Bound">h</a> <a id="1235" class="Symbol">=</a> <a id="1237" href="EquivalenceType.html#1382" class="Function">lrmap-inverse</a> <a id="1251" href="FunExtAxiom.html#749" class="Function">eqFunExt</a>
</pre>

<pre class="Agda">
  <a id="funext-η"></a><a id="1287" href="FunExtAxiom.html#1287" class="Function">funext-η</a>
    <a id="1300" class="Symbol">:</a> <a id="1302" class="Symbol">(</a><a id="1303" href="FunExtAxiom.html#1303" class="Bound">p</a> <a id="1305" class="Symbol">:</a> <a id="1307" href="FunExtAxiom.html#459" class="Bound">f</a> <a id="1309" href="EqualityType.html#931" class="Datatype Operator">==</a> <a id="1312" href="FunExtAxiom.html#461" class="Bound">g</a><a id="1313" class="Symbol">)</a>
    <a id="1319" class="Comment">------------------------</a>
    <a id="1348" class="Symbol">→</a> <a id="1350" href="FunExtAxiom.html#929" class="Function">funext</a> <a id="1357" class="Symbol">(</a><a id="1358" href="FunExtAxiom.html#545" class="Function">happly</a> <a id="1365" href="FunExtAxiom.html#1303" class="Bound">p</a><a id="1366" class="Symbol">)</a> <a id="1368" href="EqualityType.html#931" class="Datatype Operator">==</a> <a id="1371" href="FunExtAxiom.html#1303" class="Bound">p</a>

  <a id="1376" href="FunExtAxiom.html#1287" class="Function">funext-η</a> <a id="1385" href="FunExtAxiom.html#1385" class="Bound">p</a> <a id="1387" class="Symbol">=</a> <a id="1389" href="EquivalenceType.html#1609" class="Function">rlmap-inverse</a> <a id="1403" href="FunExtAxiom.html#749" class="Function">eqFunExt</a>
</pre>
