---
layout: page
title: "Function extensionality"
category: lemmas functions homotopy
toc: true
agda: true
gallery: true
latex: true
references: true
linkify: true
showcitation: true
home: true
---

<div class="hide" >
<pre class="Agda">
<a id="233" class="Symbol">{-#</a> <a id="237" class="Keyword">OPTIONS</a> <a id="245" class="Pragma">--without-K</a> <a id="257" class="Symbol">#-}</a>
<a id="261" class="Keyword">open</a> <a id="266" class="Keyword">import</a> <a id="273" href="Transport.html" class="Module">Transport</a>
<a id="283" class="Keyword">open</a> <a id="288" class="Keyword">import</a> <a id="295" href="EquivalenceType.html" class="Module">EquivalenceType</a>
<a id="311" class="Keyword">open</a> <a id="316" class="Keyword">import</a> <a id="323" href="HomotopyType.html" class="Module">HomotopyType</a>
</pre>
</div>

## Function extensionality

<pre class="Agda">

<a id="397" class="Keyword">module</a> <a id="404" href="FunExtAxiom.html" class="Module">FunExtAxiom</a> <a id="416" class="Symbol">{</a><a id="417" href="FunExtAxiom.html#417" class="Bound">ℓᵢ</a> <a id="420" href="FunExtAxiom.html#420" class="Bound">ℓⱼ</a><a id="422" class="Symbol">}</a> <a id="424" class="Symbol">{</a><a id="425" href="FunExtAxiom.html#425" class="Bound">A</a> <a id="427" class="Symbol">:</a> <a id="429" href="Intro.html#1720" class="Function">Type</a> <a id="434" href="FunExtAxiom.html#417" class="Bound">ℓᵢ</a><a id="436" class="Symbol">}</a>
  <a id="440" class="Symbol">{</a><a id="441" href="FunExtAxiom.html#441" class="Bound">B</a> <a id="443" class="Symbol">:</a> <a id="445" href="FunExtAxiom.html#425" class="Bound">A</a> <a id="447" class="Symbol">→</a> <a id="449" href="Intro.html#1720" class="Function">Type</a> <a id="454" href="FunExtAxiom.html#420" class="Bound">ℓⱼ</a><a id="456" class="Symbol">}</a> <a id="458" class="Symbol">{</a><a id="459" href="FunExtAxiom.html#459" class="Bound">f</a> <a id="461" href="FunExtAxiom.html#461" class="Bound">g</a> <a id="463" class="Symbol">:</a> <a id="465" class="Symbol">(</a><a id="466" href="FunExtAxiom.html#466" class="Bound">a</a> <a id="468" class="Symbol">:</a> <a id="470" href="FunExtAxiom.html#425" class="Bound">A</a><a id="471" class="Symbol">)</a> <a id="473" class="Symbol">→</a> <a id="475" href="FunExtAxiom.html#441" class="Bound">B</a> <a id="477" href="FunExtAxiom.html#466" class="Bound">a</a><a id="478" class="Symbol">}</a> <a id="480" class="Keyword">where</a>
</pre>

<pre class="Agda">
  <a id="513" class="Comment">-- Application of an homotopy</a>
  <a id="happly"></a><a id="545" href="FunExtAxiom.html#545" class="Function">happly</a>
    <a id="556" class="Symbol">:</a> <a id="558" href="FunExtAxiom.html#459" class="Bound">f</a> <a id="560" href="BasicTypes.html#4294" class="Datatype Operator">==</a> <a id="563" href="FunExtAxiom.html#461" class="Bound">g</a>
    <a id="569" class="Comment">------------------------</a>
    <a id="598" class="Symbol">→</a> <a id="600" class="Symbol">((</a><a id="602" href="FunExtAxiom.html#602" class="Bound">x</a> <a id="604" class="Symbol">:</a> <a id="606" href="FunExtAxiom.html#425" class="Bound">A</a><a id="607" class="Symbol">)</a> <a id="609" class="Symbol">→</a> <a id="611" href="FunExtAxiom.html#459" class="Bound">f</a> <a id="613" href="FunExtAxiom.html#602" class="Bound">x</a> <a id="615" href="BasicTypes.html#4294" class="Datatype Operator">==</a> <a id="618" href="FunExtAxiom.html#461" class="Bound">g</a> <a id="620" href="FunExtAxiom.html#602" class="Bound">x</a><a id="621" class="Symbol">)</a>

  <a id="626" href="FunExtAxiom.html#545" class="Function">happly</a> <a id="633" href="BasicTypes.html#4349" class="InductiveConstructor">idp</a> <a id="637" href="FunExtAxiom.html#637" class="Bound">x</a> <a id="639" class="Symbol">=</a> <a id="641" href="BasicTypes.html#4586" class="Function">refl</a> <a id="646" class="Symbol">(</a><a id="647" href="FunExtAxiom.html#459" class="Bound">f</a> <a id="649" href="FunExtAxiom.html#637" class="Bound">x</a><a id="650" class="Symbol">)</a>

  <a id="655" class="Comment">-- synonyms:</a>
  <a id="≡-app"></a><a id="670" href="FunExtAxiom.html#670" class="Function">≡-app</a> <a id="676" class="Symbol">=</a> <a id="678" href="FunExtAxiom.html#545" class="Function">happly</a>
</pre>

<pre class="Agda">
  <a id="712" class="Keyword">postulate</a>
    <a id="axiomFunExt"></a><a id="726" href="FunExtAxiom.html#726" class="Postulate">axiomFunExt</a> <a id="738" class="Symbol">:</a> <a id="740" href="EquivalenceType.html#939" class="Function">isEquiv</a> <a id="748" href="FunExtAxiom.html#545" class="Function">happly</a>
</pre>

<pre class="Agda">
  <a id="eqFunExt"></a><a id="782" href="FunExtAxiom.html#782" class="Function">eqFunExt</a>
    <a id="795" class="Symbol">:</a> <a id="797" class="Symbol">(</a><a id="798" href="FunExtAxiom.html#459" class="Bound">f</a> <a id="800" href="BasicTypes.html#4294" class="Datatype Operator">==</a> <a id="803" href="FunExtAxiom.html#461" class="Bound">g</a><a id="804" class="Symbol">)</a> <a id="806" href="EquivalenceType.html#1095" class="Function Operator">≃</a> <a id="808" class="Symbol">((</a><a id="810" href="FunExtAxiom.html#810" class="Bound">x</a> <a id="812" class="Symbol">:</a> <a id="814" href="FunExtAxiom.html#425" class="Bound">A</a><a id="815" class="Symbol">)</a> <a id="817" class="Symbol">→</a> <a id="819" href="FunExtAxiom.html#459" class="Bound">f</a> <a id="821" href="FunExtAxiom.html#810" class="Bound">x</a> <a id="823" href="BasicTypes.html#4294" class="Datatype Operator">==</a> <a id="826" href="FunExtAxiom.html#461" class="Bound">g</a> <a id="828" href="FunExtAxiom.html#810" class="Bound">x</a><a id="829" class="Symbol">)</a>

  <a id="834" href="FunExtAxiom.html#782" class="Function">eqFunExt</a> <a id="843" class="Symbol">=</a> <a id="845" href="FunExtAxiom.html#545" class="Function">happly</a> <a id="852" href="BasicTypes.html#1582" class="InductiveConstructor Operator">,</a> <a id="854" href="FunExtAxiom.html#726" class="Postulate">axiomFunExt</a>
</pre>

<pre class="Agda">
  <a id="893" class="Comment">-- From this, the usual notion of function extensionality follows.</a>
  <a id="funext"></a><a id="962" href="FunExtAxiom.html#962" class="Function">funext</a>
    <a id="973" class="Symbol">:</a> <a id="975" class="Symbol">((</a><a id="977" href="FunExtAxiom.html#977" class="Bound">x</a> <a id="979" class="Symbol">:</a> <a id="981" href="FunExtAxiom.html#425" class="Bound">A</a><a id="982" class="Symbol">)</a> <a id="984" class="Symbol">→</a> <a id="986" href="FunExtAxiom.html#459" class="Bound">f</a> <a id="988" href="FunExtAxiom.html#977" class="Bound">x</a> <a id="990" href="BasicTypes.html#4294" class="Datatype Operator">==</a> <a id="993" href="FunExtAxiom.html#461" class="Bound">g</a> <a id="995" href="FunExtAxiom.html#977" class="Bound">x</a><a id="996" class="Symbol">)</a>
    <a id="1002" class="Comment">------------------------</a>
    <a id="1031" class="Symbol">→</a> <a id="1033" href="FunExtAxiom.html#459" class="Bound">f</a> <a id="1035" href="BasicTypes.html#4294" class="Datatype Operator">==</a> <a id="1038" href="FunExtAxiom.html#461" class="Bound">g</a>

  <a id="1043" href="FunExtAxiom.html#962" class="Function">funext</a> <a id="1050" class="Symbol">=</a> <a id="1052" href="EquivalenceType.html#1464" class="Function">remap</a> <a id="1058" href="FunExtAxiom.html#782" class="Function">eqFunExt</a>
</pre>

<pre class="Agda">
  <a id="1094" class="Comment">-- Beta and eta rules for function extensionality</a>
  <a id="funext-β"></a><a id="1146" href="FunExtAxiom.html#1146" class="Function">funext-β</a>
    <a id="1159" class="Symbol">:</a> <a id="1161" class="Symbol">(</a><a id="1162" href="FunExtAxiom.html#1162" class="Bound">h</a> <a id="1164" class="Symbol">:</a> <a id="1166" class="Symbol">((</a><a id="1168" href="FunExtAxiom.html#1168" class="Bound">x</a> <a id="1170" class="Symbol">:</a> <a id="1172" href="FunExtAxiom.html#425" class="Bound">A</a><a id="1173" class="Symbol">)</a> <a id="1175" class="Symbol">→</a> <a id="1177" href="FunExtAxiom.html#459" class="Bound">f</a> <a id="1179" href="FunExtAxiom.html#1168" class="Bound">x</a> <a id="1181" href="BasicTypes.html#4294" class="Datatype Operator">==</a> <a id="1184" href="FunExtAxiom.html#461" class="Bound">g</a> <a id="1186" href="FunExtAxiom.html#1168" class="Bound">x</a><a id="1187" class="Symbol">))</a>
    <a id="1194" class="Comment">------------------------------</a>
    <a id="1229" class="Symbol">→</a> <a id="1231" href="FunExtAxiom.html#545" class="Function">happly</a> <a id="1238" class="Symbol">(</a><a id="1239" href="FunExtAxiom.html#962" class="Function">funext</a> <a id="1246" href="FunExtAxiom.html#1162" class="Bound">h</a><a id="1247" class="Symbol">)</a> <a id="1249" href="BasicTypes.html#4294" class="Datatype Operator">==</a> <a id="1252" href="FunExtAxiom.html#1162" class="Bound">h</a>

  <a id="1257" href="FunExtAxiom.html#1146" class="Function">funext-β</a> <a id="1266" href="FunExtAxiom.html#1266" class="Bound">h</a> <a id="1268" class="Symbol">=</a> <a id="1270" href="EquivalenceType.html#1699" class="Function">lrmap-inverse</a> <a id="1284" href="FunExtAxiom.html#782" class="Function">eqFunExt</a>
</pre>

<pre class="Agda">
  <a id="funext-η"></a><a id="1320" href="FunExtAxiom.html#1320" class="Function">funext-η</a>
    <a id="1333" class="Symbol">:</a> <a id="1335" class="Symbol">(</a><a id="1336" href="FunExtAxiom.html#1336" class="Bound">p</a> <a id="1338" class="Symbol">:</a> <a id="1340" href="FunExtAxiom.html#459" class="Bound">f</a> <a id="1342" href="BasicTypes.html#4294" class="Datatype Operator">==</a> <a id="1345" href="FunExtAxiom.html#461" class="Bound">g</a><a id="1346" class="Symbol">)</a>
    <a id="1352" class="Comment">------------------------</a>
    <a id="1381" class="Symbol">→</a> <a id="1383" href="FunExtAxiom.html#962" class="Function">funext</a> <a id="1390" class="Symbol">(</a><a id="1391" href="FunExtAxiom.html#545" class="Function">happly</a> <a id="1398" href="FunExtAxiom.html#1336" class="Bound">p</a><a id="1399" class="Symbol">)</a> <a id="1401" href="BasicTypes.html#4294" class="Datatype Operator">==</a> <a id="1404" href="FunExtAxiom.html#1336" class="Bound">p</a>

  <a id="1409" href="FunExtAxiom.html#1320" class="Function">funext-η</a> <a id="1418" href="FunExtAxiom.html#1418" class="Bound">p</a> <a id="1420" class="Symbol">=</a> <a id="1422" href="EquivalenceType.html#1926" class="Function">rlmap-inverse</a> <a id="1436" href="FunExtAxiom.html#782" class="Function">eqFunExt</a>
</pre>
